Makefile
@@ -91,6 +91,8 @@ BACKEND=\
   SelectLongproof.v Selectionproof.v \
   Registers.v RTL.v \
   RTLgen.v RTLgenspec.v RTLgenproof.v \
+  Tailcall.v Tailcallproof.v \
+  Inlining.v Inliningspec.v Inliningproof.v \
   Renumber.v Renumberproof.v \
   RTLtyping.v \
   Kildall.v Liveness.v \
